CoqOfRust/core/cmp.v
@@ -32,11 +32,15 @@ Traits
 [x] PartialOrd
 *)
 Module PartialEq.
-  Class Trait (Self : Set) {Rhs : option Set} : Set := {
-    Rhs := defaultType Rhs Self;
+  Class Trait (Self : Set) {Rhs : Set} : Set := {
+    Rhs := Rhs;
 
     eq `{State.Trait} : ref Self -> ref Rhs -> M bool;
   }.
+
+  Module Default.
+    Definition Rhs (Self : Set) : Set := Self.
+  End Default.
 
   Global Instance Method_eq `{State.Trait} `(Trait) : Notation.Dot "eq" := {
     Notation.dot := eq;
@@ -48,13 +52,13 @@ Module PartialEq.
   }.
 
   Module Impl_PartialEq_for_str.
-    Global Instance I : Trait str (Rhs := None). Admitted.
+    Global Instance I : Trait str (Rhs := Default.Rhs str). Admitted.
   End Impl_PartialEq_for_str.
 End PartialEq.
 
 Module PartialOrd.
-  Class Trait (Self : Set) (Rhs : option Set) : Set := {
-    Rhs := defaultType Rhs Self;
+  Class Trait (Self : Set) {Rhs : Set} : Set := {
+    Rhs := Rhs;
     partial_cmp `{State.Trait} :
       ref Self -> ref Self -> M (core.option.Option (Ordering.t));
 
@@ -63,6 +67,10 @@ Module PartialOrd.
     gt `{State.Trait} : ref Self -> ref Rhs -> M bool;
     ge `{State.Trait} : ref Self -> ref Rhs -> M bool; *)
   }.
+
+  Module Default.
+    Definition Rhs (Self : Set) : Set := Self.
+  End Default.
 
   Global Instance Method_partial_cmp `{State.Trait} `(Trait) :
     Notation.Dot "partial_cmp" := {
@@ -81,8 +89,7 @@ Module PartialOrd.
     Notation.dot := ge;
   }. *)
   Module Impl_PartialOrd_for_str.
-    Global Instance I : Trait str None. Admitted.
-    Global Instance I' : Trait str (Some str). Admitted.
+    Global Instance I : Trait str (Rhs := str). Admitted.
   End Impl_PartialOrd_for_str.
 End PartialOrd.
 
@@ -91,7 +98,8 @@ pub trait Eq: PartialEq<Self> { }
  *)
 Module Eq.
   Unset Primitive Projections.
-  Class Trait (Self : Set) `{PartialEq.Trait Self (Rhs := None)} : Set := { }.
+  Class Trait (Self : Set)
+    `{PartialEq.Trait Self (Rhs := PartialEq.Default.Rhs Self)} : Set := { }.
   Set Primitive Projections.
 
   Module Impl_Eq_for_str.
@@ -116,11 +124,11 @@ pub trait Ord: Eq + PartialOrd<Self> {
 Module Ord.
   Class Trait (Self : Set) 
     `{Eq.Trait Self}
-    `{PartialOrd.Trait Self (Some Self)} :={
+    `{PartialOrd.Trait Self (Rhs := Self)} :={
     cmp : ref Self -> ref Self -> Ordering;
     max : Self -> Self -> Self;
     min : Self -> Self -> Self;
-    clamp `{PartialOrd.Trait Self (Some Self)} : Self -> Self -> Self;
+    clamp `{PartialOrd.Trait Self (Rhs := Self)} : Self -> Self -> Self;
 
     }.
 
@@ -159,7 +167,8 @@ Module Impls.
   Module Impl_PartialEq_for_unit.
     Definition eq `{State.Trait} (x y : unit) : M bool := Pure true.
 
-    Global Instance I : PartialEq.Trait unit (Rhs := None) := {
+    Global Instance I :
+      PartialEq.Trait unit (Rhs := PartialEq.Default.Rhs unit) := {
       eq `{State.Trait} := eq;
     }.
   End Impl_PartialEq_for_unit.
