CoqOfRust/ink/erc20.v
@@ -5,7 +5,6 @@ Require CoqOfRust.ink.ink_storage.
 Require CoqOfRust.ink.ink_env.
 Require CoqOfRust.ink.ink.
 
-
 Module erc20.
   Module Erc20.
     Unset Primitive Projections.
@@ -73,7 +72,10 @@ Module erc20.
   Definition ChainExtension : Set := ink_env.types.Environment.ChainExtension.
   
   Definition MAX_EVENT_TOPICS `{H' : State.Trait} : usize :=
-    run (Pure ink_env.types.Environment.MAX_EVENT_TOPICS).
+    run
+      (Pure
+        (ink_env.types.Environment.MAX_EVENT_TOPICS
+          (Self := ink_env.contract.ContractEnv.Env))).
   
   Module Impl_core_default_Default_for_erc20_erc20_Erc20.
     Definition Self := erc20.erc20.Erc20.
@@ -208,7 +210,10 @@ Module erc20.
     Definition Error : Set := ink.reflect.dispatch.ConstructorOutput.Error.
     
     Definition
-      IS_RESULT `{State.Trait} := Pure ink.reflect.dispatch.ConstructorOutput.IS_RESULT.
+      IS_RESULT
+      `{H' : State.Trait} := Pure
+        (ink.reflect.dispatch.ConstructorOutput.IS_RESULT
+          (Self := (ink.reflect.dispatch.ConstructorOutputValue Self))).
     
     Global Instance AssociatedFunction_IS_RESULT `{H' : State.Trait} :
       Notation.DoubleColon Self "IS_RESULT" := {
@@ -216,7 +221,8 @@ Module erc20.
     }.
     
     Definition
-      CALLABLE `{State.Trait} := Pure
+      CALLABLE
+      `{H' : State.Trait} := Pure
         (fun __ink_binding_0 => erc20.erc20.Erc20::["new"] __ink_binding_0).
     
     Global Instance AssociatedFunction_CALLABLE `{H' : State.Trait} :
@@ -224,21 +230,21 @@ Module erc20.
       Notation.double_colon := CALLABLE;
     }.
     
-    Definition PAYABLE `{State.Trait} := Pure false.
+    Definition PAYABLE `{H' : State.Trait} := Pure false.
     
     Global Instance AssociatedFunction_PAYABLE `{H' : State.Trait} :
       Notation.DoubleColon Self "PAYABLE" := {
       Notation.double_colon := PAYABLE;
     }.
     
-    Definition SELECTOR `{State.Trait} := Pure [ 155; 174; 157; 94 ].
+    Definition SELECTOR `{H' : State.Trait} := Pure [ 155; 174; 157; 94 ].
     
     Global Instance AssociatedFunction_SELECTOR `{H' : State.Trait} :
       Notation.DoubleColon Self "SELECTOR" := {
       Notation.double_colon := SELECTOR;
     }.
     
-    Definition LABEL `{State.Trait} := Pure "new".
+    Definition LABEL `{H' : State.Trait} := Pure "new".
     
     Global Instance AssociatedFunction_LABEL `{H' : State.Trait} :
       Notation.DoubleColon Self "LABEL" := {
@@ -286,7 +292,8 @@ Module erc20.
     Definition Storage : Set := erc20.erc20.Erc20.
     
     Definition
-      CALLABLE `{State.Trait} := Pure
+      CALLABLE
+      `{H' : State.Trait} := Pure
         (fun storage _ => erc20.erc20.Erc20::["total_supply"] storage).
     
     Global Instance AssociatedFunction_CALLABLE `{H' : State.Trait} :
@@ -294,28 +301,28 @@ Module erc20.
       Notation.double_colon := CALLABLE;
     }.
     
-    Definition SELECTOR `{State.Trait} := Pure [ 219; 99; 117; 168 ].
+    Definition SELECTOR `{H' : State.Trait} := Pure [ 219; 99; 117; 168 ].
     
     Global Instance AssociatedFunction_SELECTOR `{H' : State.Trait} :
       Notation.DoubleColon Self "SELECTOR" := {
       Notation.double_colon := SELECTOR;
     }.
     
-    Definition PAYABLE `{State.Trait} := Pure false.
+    Definition PAYABLE `{H' : State.Trait} := Pure false.
     
     Global Instance AssociatedFunction_PAYABLE `{H' : State.Trait} :
       Notation.DoubleColon Self "PAYABLE" := {
       Notation.double_colon := PAYABLE;
     }.
     
-    Definition MUTATES := Pure false.
+    Definition MUTATES `{H' : State.Trait} := Pure false.
     
     Global Instance AssociatedFunction_MUTATES `{H' : State.Trait} :
       Notation.DoubleColon Self "MUTATES" := {
       Notation.double_colon := MUTATES;
     }.
     
-    Definition LABEL := Pure "total_supply".
+    Definition LABEL `{H' : State.Trait} := Pure "total_supply".
     
     Global Instance AssociatedFunction_LABEL `{H' : State.Trait} :
       Notation.DoubleColon Self "LABEL" := {
@@ -357,7 +364,8 @@ Module erc20.
     Definition Storage : Set := erc20.erc20.Erc20.
     
     Definition
-      CALLABLE `{State.Trait} := Pure
+      CALLABLE
+      `{H' : State.Trait} := Pure
         (fun storage __ink_binding_0 =>
           erc20.erc20.Erc20::["balance_of"] storage __ink_binding_0).
     
@@ -366,28 +374,28 @@ Module erc20.
       Notation.double_colon := CALLABLE;
     }.
     
-    Definition SELECTOR `{State.Trait} := Pure [ 15; 117; 90; 86 ].
+    Definition SELECTOR `{H' : State.Trait} := Pure [ 15; 117; 90; 86 ].
     
     Global Instance AssociatedFunction_SELECTOR `{H' : State.Trait} :
       Notation.DoubleColon Self "SELECTOR" := {
       Notation.double_colon := SELECTOR;
     }.
     
-    Definition PAYABLE `{State.Trait} := Pure false.
+    Definition PAYABLE `{H' : State.Trait} := Pure false.
     
     Global Instance AssociatedFunction_PAYABLE `{H' : State.Trait} :
       Notation.DoubleColon Self "PAYABLE" := {
       Notation.double_colon := PAYABLE;
     }.
     
-    Definition MUTATES := Pure false.
+    Definition MUTATES `{H' : State.Trait} := Pure false.
     
     Global Instance AssociatedFunction_MUTATES `{H' : State.Trait} :
       Notation.DoubleColon Self "MUTATES" := {
       Notation.double_colon := MUTATES;
     }.
     
-    Definition LABEL := Pure "balance_of".
+    Definition LABEL `{H' : State.Trait} := Pure "balance_of".
     
     Global Instance AssociatedFunction_LABEL `{H' : State.Trait} :
       Notation.DoubleColon Self "LABEL" := {
@@ -429,7 +437,8 @@ Module erc20.
     Definition Storage : Set := erc20.erc20.Erc20.
     
     Definition
-      CALLABLE `{State.Trait} := Pure
+      CALLABLE
+      `{H' : State.Trait} := Pure
         (fun storage (__ink_binding_0, __ink_binding_1) =>
           erc20.erc20.Erc20::["allowance"]
             storage
@@ -441,28 +450,28 @@ Module erc20.
       Notation.double_colon := CALLABLE;
     }.
     
-    Definition SELECTOR `{State.Trait} := Pure [ 106; 0; 22; 94 ].
+    Definition SELECTOR `{H' : State.Trait} := Pure [ 106; 0; 22; 94 ].
     
     Global Instance AssociatedFunction_SELECTOR `{H' : State.Trait} :
       Notation.DoubleColon Self "SELECTOR" := {
       Notation.double_colon := SELECTOR;
     }.
     
-    Definition PAYABLE `{State.Trait} := Pure false.
+    Definition PAYABLE `{H' : State.Trait} := Pure false.
     
     Global Instance AssociatedFunction_PAYABLE `{H' : State.Trait} :
       Notation.DoubleColon Self "PAYABLE" := {
       Notation.double_colon := PAYABLE;
     }.
     
-    Definition MUTATES := Pure false.
+    Definition MUTATES `{H' : State.Trait} := Pure false.
     
     Global Instance AssociatedFunction_MUTATES `{H' : State.Trait} :
       Notation.DoubleColon Self "MUTATES" := {
       Notation.double_colon := MUTATES;
     }.
     
-    Definition LABEL := Pure "allowance".
+    Definition LABEL `{H' : State.Trait} := Pure "allowance".
     
     Global Instance AssociatedFunction_LABEL `{H' : State.Trait} :
       Notation.DoubleColon Self "LABEL" := {
@@ -504,7 +513,8 @@ Module erc20.
     Definition Storage : Set := erc20.erc20.Erc20.
     
     Definition
-      CALLABLE `{State.Trait} := Pure
+      CALLABLE
+      `{H' : State.Trait} := Pure
         (fun storage (__ink_binding_0, __ink_binding_1) =>
           erc20.erc20.Erc20::["transfer"]
             storage
@@ -516,28 +526,28 @@ Module erc20.
       Notation.double_colon := CALLABLE;
     }.
     
-    Definition SELECTOR `{State.Trait} := Pure [ 132; 161; 93; 161 ].
+    Definition SELECTOR `{H' : State.Trait} := Pure [ 132; 161; 93; 161 ].
     
     Global Instance AssociatedFunction_SELECTOR `{H' : State.Trait} :
       Notation.DoubleColon Self "SELECTOR" := {
       Notation.double_colon := SELECTOR;
     }.
     
-    Definition PAYABLE `{State.Trait} := Pure false.
+    Definition PAYABLE `{H' : State.Trait} := Pure false.
     
     Global Instance AssociatedFunction_PAYABLE `{H' : State.Trait} :
       Notation.DoubleColon Self "PAYABLE" := {
       Notation.double_colon := PAYABLE;
     }.
     
-    Definition MUTATES := Pure true.
+    Definition MUTATES `{H' : State.Trait} := Pure true.
     
     Global Instance AssociatedFunction_MUTATES `{H' : State.Trait} :
       Notation.DoubleColon Self "MUTATES" := {
       Notation.double_colon := MUTATES;
     }.
     
-    Definition LABEL := Pure "transfer".
+    Definition LABEL `{H' : State.Trait} := Pure "transfer".
     
     Global Instance AssociatedFunction_LABEL `{H' : State.Trait} :
       Notation.DoubleColon Self "LABEL" := {
@@ -579,7 +589,8 @@ Module erc20.
     Definition Storage : Set := erc20.erc20.Erc20.
     
     Definition
-      CALLABLE `{State.Trait} := Pure
+      CALLABLE
+      `{H' : State.Trait} := Pure
         (fun storage (__ink_binding_0, __ink_binding_1) =>
           erc20.erc20.Erc20::["approve"]
             storage
@@ -591,28 +602,28 @@ Module erc20.
       Notation.double_colon := CALLABLE;
     }.
     
-    Definition SELECTOR `{State.Trait} := Pure [ 104; 18; 102; 160 ].
+    Definition SELECTOR `{H' : State.Trait} := Pure [ 104; 18; 102; 160 ].
     
     Global Instance AssociatedFunction_SELECTOR `{H' : State.Trait} :
       Notation.DoubleColon Self "SELECTOR" := {
       Notation.double_colon := SELECTOR;
     }.
     
-    Definition PAYABLE `{State.Trait} := Pure false.
+    Definition PAYABLE `{H' : State.Trait} := Pure false.
     
     Global Instance AssociatedFunction_PAYABLE `{H' : State.Trait} :
       Notation.DoubleColon Self "PAYABLE" := {
       Notation.double_colon := PAYABLE;
     }.
     
-    Definition MUTATES := Pure true.
+    Definition MUTATES `{H' : State.Trait} := Pure true.
     
     Global Instance AssociatedFunction_MUTATES `{H' : State.Trait} :
       Notation.DoubleColon Self "MUTATES" := {
       Notation.double_colon := MUTATES;
     }.
     
-    Definition LABEL := Pure "approve".
+    Definition LABEL `{H' : State.Trait} := Pure "approve".
     
     Global Instance AssociatedFunction_LABEL `{H' : State.Trait} :
       Notation.DoubleColon Self "LABEL" := {
@@ -655,7 +666,8 @@ Module erc20.
     Definition Storage : Set := erc20.erc20.Erc20.
     
     Definition
-      CALLABLE `{State.Trait} := Pure
+      CALLABLE
+      `{H' : State.Trait} := Pure
         (fun storage (__ink_binding_0, __ink_binding_1, __ink_binding_2) =>
           erc20.erc20.Erc20::["transfer_from"]
             storage
@@ -668,28 +680,28 @@ Module erc20.
       Notation.double_colon := CALLABLE;
     }.
     
-    Definition SELECTOR `{State.Trait} := Pure [ 11; 57; 111; 24 ].
+    Definition SELECTOR `{H' : State.Trait} := Pure [ 11; 57; 111; 24 ].
     
     Global Instance AssociatedFunction_SELECTOR `{H' : State.Trait} :
       Notation.DoubleColon Self "SELECTOR" := {
       Notation.double_colon := SELECTOR;
     }.
     
-    Definition PAYABLE `{State.Trait} := Pure false.
+    Definition PAYABLE `{H' : State.Trait} := Pure false.
     
     Global Instance AssociatedFunction_PAYABLE `{H' : State.Trait} :
       Notation.DoubleColon Self "PAYABLE" := {
       Notation.double_colon := PAYABLE;
     }.
     
-    Definition MUTATES := Pure true.
+    Definition MUTATES `{H' : State.Trait} := Pure true.
     
     Global Instance AssociatedFunction_MUTATES `{H' : State.Trait} :
       Notation.DoubleColon Self "MUTATES" := {
       Notation.double_colon := MUTATES;
     }.
     
-    Definition LABEL := Pure "transfer_from".
+    Definition LABEL `{H' : State.Trait} := Pure "transfer_from".
     
     Global Instance AssociatedFunction_LABEL `{H' : State.Trait} :
       Notation.DoubleColon Self "LABEL" := {
@@ -816,7 +828,10 @@ Module erc20.
       Notation.dot := eq;
     }.
     
-    Global Instance I : core.cmp.PartialEq.Trait Self (Rhs := None) := {
+    Global Instance I
+      : core.cmp.PartialEq.Trait Self
+          (Rhs := core.cmp.PartialEq.Default.Rhs Self)
+        := {
       core.cmp.PartialEq.eq `{H' : State.Trait} := eq;
     }.
     Global Hint Resolve I : core.
@@ -936,7 +951,9 @@ Module erc20.
         (self : ref Self)
         : M (H := H') (ink_primitives.MessageResult erc20.erc20.Balance) :=
       let* α0 :=
-        ink.codegen.trait_def.call_builder.TraitCallBuilder.call self in
+        (ink.codegen.trait_def.call_builder.TraitCallBuilder.call
+            (Self := Self))
+          self in
       let* α1 := α0.["total_supply"] in
       let* α2 := α1.["try_invoke"] in
       α2.["unwrap_or_else"]
@@ -981,7 +998,9 @@ Module erc20.
         (owner : erc20.erc20.AccountId)
         : M (H := H') (ink_primitives.MessageResult erc20.erc20.Balance) :=
       let* α0 :=
-        ink.codegen.trait_def.call_builder.TraitCallBuilder.call self in
+        (ink.codegen.trait_def.call_builder.TraitCallBuilder.call
+            (Self := Self))
+          self in
       let* α1 := α0.["balance_of"] owner in
       let* α2 := α1.["try_invoke"] in
       α2.["unwrap_or_else"]
@@ -1027,7 +1046,9 @@ Module erc20.
         (spender : erc20.erc20.AccountId)
         : M (H := H') (ink_primitives.MessageResult erc20.erc20.Balance) :=
       let* α0 :=
-        ink.codegen.trait_def.call_builder.TraitCallBuilder.call self in
+        (ink.codegen.trait_def.call_builder.TraitCallBuilder.call
+            (Self := Self))
+          self in
       let* α1 := α0.["allowance"] owner spender in
       let* α2 := α1.["try_invoke"] in
       α2.["unwrap_or_else"]
@@ -1074,7 +1095,9 @@ Module erc20.
           M (H := H')
             (ink_primitives.MessageResult (erc20.erc20.Result unit)) :=
       let* α0 :=
-        ink.codegen.trait_def.call_builder.TraitCallBuilder.call_mut self in
+        (ink.codegen.trait_def.call_builder.TraitCallBuilder.call_mut
+            (Self := Self))
+          self in
       let* α1 := α0.["transfer"] to value in
       let* α2 := α1.["try_invoke"] in
       α2.["unwrap_or_else"]
@@ -1121,7 +1144,9 @@ Module erc20.
           M (H := H')
             (ink_primitives.MessageResult (erc20.erc20.Result unit)) :=
       let* α0 :=
-        ink.codegen.trait_def.call_builder.TraitCallBuilder.call_mut self in
+        (ink.codegen.trait_def.call_builder.TraitCallBuilder.call_mut
+            (Self := Self))
+          self in
       let* α1 := α0.["approve"] spender value in
       let* α2 := α1.["try_invoke"] in
       α2.["unwrap_or_else"]
@@ -1171,7 +1196,9 @@ Module erc20.
           M (H := H')
             (ink_primitives.MessageResult (erc20.erc20.Result unit)) :=
       let* α0 :=
-        ink.codegen.trait_def.call_builder.TraitCallBuilder.call_mut self in
+        (ink.codegen.trait_def.call_builder.TraitCallBuilder.call_mut
+            (Self := Self))
+          self in
       let* α1 := α0.["transfer_from"] from to value in
       let* α2 := α1.["try_invoke"] in
       α2.["unwrap_or_else"]
@@ -1199,7 +1226,9 @@ Module erc20.
         (account_id : erc20.erc20.AccountId)
         : M (H := H') Self :=
       let* α0 :=
-        ink_env.call.create_builder.FromAccountId.from_account_id account_id in
+        (ink_env.call.create_builder.FromAccountId.from_account_id
+            (Self := ink.codegen.dispatch.info.ContractCallBuilder.Type_))
+          account_id in
       Pure {| Self.inner := α0; |}.
     
     Global Instance AssociatedFunction_from_account_id `{H' : State.Trait} :
@@ -1226,7 +1255,9 @@ Module erc20.
         `{H' : State.Trait}
         (self : ref Self)
         : M (H := H') erc20.erc20.AccountId :=
-      ink.contract_ref.ToAccountId.to_account_id (addr_of self.["inner"]).
+      (ink.contract_ref.ToAccountId.to_account_id
+          (Self := ink.codegen.dispatch.info.ContractCallBuilder.Type_))
+        (addr_of self.["inner"]).
     
     Global Instance Method_to_account_id `{H' : State.Trait} :
       Notation.Dot "to_account_id" := {
@@ -1250,7 +1281,7 @@ Module erc20.
         `{H' : State.Trait}
         (self : ref Self)
         : M (H := H') (ref erc20.erc20.AccountId) :=
-      core.convert.AsRef.as_ref (addr_of self.["inner"]).
+      (core.convert.AsRef.as_ref (Self := _)) (addr_of self.["inner"]).
     
     Global Instance Method_as_ref `{H' : State.Trait} :
       Notation.Dot "as_ref" := {
@@ -1271,7 +1302,7 @@ Module erc20.
         `{H' : State.Trait}
         (self : mut_ref Self)
         : M (H := H') (mut_ref erc20.erc20.AccountId) :=
-      core.convert.AsMut.as_mut (addr_of self.["inner"]).
+      (core.convert.AsMut.as_mut (Self := _)) (addr_of self.["inner"]).
     
     Global Instance Method_as_mut `{H' : State.Trait} :
       Notation.Dot "as_mut" := {
@@ -1343,7 +1374,10 @@ Module erc20.
       Notation.dot := eq;
     }.
     
-    Global Instance I : core.cmp.PartialEq.Trait Self (Rhs := None) := {
+    Global Instance I
+      : core.cmp.PartialEq.Trait Self
+          (Rhs := core.cmp.PartialEq.Default.Rhs Self)
+        := {
       core.cmp.PartialEq.eq `{H' : State.Trait} := eq;
     }.
     Global Hint Resolve I : core.
@@ -1406,7 +1440,10 @@ Definition BlockNumber : Set := ink_env.types.Environment.BlockNumber.
 Definition ChainExtension : Set := ink_env.types.Environment.ChainExtension.
 
 Definition MAX_EVENT_TOPICS `{H' : State.Trait} : usize :=
-  run (Pure ink_env.types.Environment.MAX_EVENT_TOPICS).
+  run
+    (Pure
+      (ink_env.types.Environment.MAX_EVENT_TOPICS
+        (Self := ink_env.contract.ContractEnv.Env))).
 
 Module Check.
   Unset Primitive Projections.
@@ -1507,7 +1544,10 @@ End Impl_ink_storage_traits_storage_StorableHint_for_erc20_erc20_Erc20.
 Module Impl_ink_storage_traits_storage_StorageKey_for_erc20_erc20_Erc20.
   Definition Self := erc20.erc20.Erc20.
   
-  Definition KEY := Pure ink_storage_traits.storage.StorageKey.KEY.
+  Definition
+    KEY
+    `{H' : State.Trait} := Pure
+      (ink_storage_traits.storage.StorageKey.KEY (Self := unit)).
   
   Global Instance AssociatedFunction_KEY `{H' : State.Trait} :
     Notation.DoubleColon Self "KEY" := {
@@ -1529,7 +1569,10 @@ Module Impl_ink_storage_traits_storage_Storable_for_erc20_erc20_Erc20.
       `{parity_scale_codec.codec.Input.Trait __ink_I}
       (__input : mut_ref __ink_I)
       : M (H := H') (core.result.Result Self parity_scale_codec.error.Error) :=
-    let* α0 := ink_storage_traits.storage.Storable.decode __input in
+    let* α0 :=
+      (ink_storage_traits.storage.Storable.decode
+          (Self := ink_storage_traits.storage.AutoStorableHint.Type_))
+        __input in
     let* α1 := α0.["branch"] in
     let* α2 :=
       match α1 with
@@ -1538,7 +1581,10 @@ Module Impl_ink_storage_traits_storage_Storable_for_erc20_erc20_Erc20.
         Return α0
       | LanguageItem.Continue val => Pure val
       end in
-    let* α3 := ink_storage_traits.storage.Storable.decode __input in
+    let* α3 :=
+      (ink_storage_traits.storage.Storable.decode
+          (Self := ink_storage_traits.storage.AutoStorableHint.Type_))
+        __input in
     let* α4 := α3.["branch"] in
     let* α5 :=
       match α4 with
@@ -1547,7 +1593,10 @@ Module Impl_ink_storage_traits_storage_Storable_for_erc20_erc20_Erc20.
         Return α0
       | LanguageItem.Continue val => Pure val
       end in
-    let* α6 := ink_storage_traits.storage.Storable.decode __input in
+    let* α6 :=
+      (ink_storage_traits.storage.Storable.decode
+          (Self := ink_storage_traits.storage.AutoStorableHint.Type_))
+        __input in
     let* α7 := α6.["branch"] in
     let* α8 :=
       match α7 with
@@ -1683,11 +1732,20 @@ Module Impl_ink_storage_traits_layout_StorageLayout_for_erc20_erc20_Erc20.
       `{H' : State.Trait}
       (__key : ref ink_primitives.key.Key)
       : M (H := H') ink_metadata.layout.Layout :=
-    let* α0 := ink_storage_traits.layout.StorageLayout.layout __key in
+    let* α0 :=
+      (ink_storage_traits.layout.StorageLayout.layout
+          (Self := ink_storage_traits.storage.AutoStorableHint.Type_))
+        __key in
     let* α1 := ink_metadata.layout.FieldLayout::["new"] "total_supply" α0 in
-    let* α2 := ink_storage_traits.layout.StorageLayout.layout __key in
+    let* α2 :=
+      (ink_storage_traits.layout.StorageLayout.layout
+          (Self := ink_storage_traits.storage.AutoStorableHint.Type_))
+        __key in
     let* α3 := ink_metadata.layout.FieldLayout::["new"] "balances" α2 in
-    let* α4 := ink_storage_traits.layout.StorageLayout.layout __key in
+    let* α4 :=
+      (ink_storage_traits.layout.StorageLayout.layout
+          (Self := ink_storage_traits.storage.AutoStorableHint.Type_))
+        __key in
     let* α5 := ink_metadata.layout.FieldLayout::["new"] "allowances" α4 in
     let* α6 :=
       ink_metadata.layout.StructLayout::["new"] "Erc20" [ α1; α3; α5 ] in
@@ -1734,7 +1792,7 @@ End Impl_core_default_Default_for_erc20_erc20_Erc20.
 Module Impl_ink_reflect_contract_ContractName_for_erc20_erc20_Erc20.
   Definition Self := erc20.erc20.Erc20.
   
-  Definition NAME := Pure "Erc20".
+  Definition NAME `{H' : State.Trait} := Pure "Erc20".
   
   Global Instance AssociatedFunction_NAME `{H' : State.Trait} :
     Notation.DoubleColon Self "NAME" := {
@@ -1754,7 +1812,7 @@ Module Impl_ink_codegen_env_Env_for_StaticRef_erc20_erc20_Erc20.
     ink.env_access.EnvAccess ink_env.contract.ContractEnv.Env.
   
   Definition env `{H' : State.Trait} (self : Self) : M (H := H') EnvAccess :=
-    core.default.Default.default.
+    (core.default.Default.default (Self := ink.codegen.env.Env.EnvAccess)).
   
   Global Instance Method_env `{H' : State.Trait} : Notation.Dot "env" := {
     Notation.dot := env;
@@ -1774,7 +1832,8 @@ Module Impl_ink_codegen_env_StaticEnv_for_erc20_erc20_Erc20.
     ink.env_access.EnvAccess ink_env.contract.ContractEnv.Env.
   
   Definition env `{H' : State.Trait} : M (H := H') EnvAccess :=
-    core.default.Default.default.
+    (core.default.Default.default
+        (Self := ink.codegen.env.StaticEnv.EnvAccess)).
   
   Global Instance AssociatedFunction_env `{H' : State.Trait} :
     Notation.DoubleColon Self "env" := {
@@ -1870,7 +1929,8 @@ Module
   Definition Self := erc20.erc20.__ink_EventBase.
   
   Global Instance I
-    : parity_scale_codec.encode_like.EncodeLike.Trait Self (T := None)
+    : parity_scale_codec.encode_like.EncodeLike.Trait Self
+        (T := parity_scale_codec.encode_like.EncodeLike.Default.T Self)
       := parity_scale_codec.encode_like.EncodeLike.Build_Trait _.
   Global Hint Resolve I : core.
 End
@@ -1905,7 +1965,9 @@ Module Impl_parity_scale_codec_codec_Decode_for_erc20_erc20___ink_EventBase.
         let* α0 :=
           (fun  =>
               let* __codec_res_edqy :=
-                parity_scale_codec.codec.Decode.decode __codec_input_edqy in
+                (parity_scale_codec.codec.Decode.decode
+                    (Self := erc20.erc20.Transfer))
+                  __codec_input_edqy in
               let* α0 :=
                 match __codec_res_edqy with
                 | core.result.Result.Err e =>
@@ -1926,7 +1988,9 @@ Module Impl_parity_scale_codec_codec_Decode_for_erc20_erc20___ink_EventBase.
         let* α0 :=
           (fun  =>
               let* __codec_res_edqy :=
-                parity_scale_codec.codec.Decode.decode __codec_input_edqy in
+                (parity_scale_codec.codec.Decode.decode
+                    (Self := erc20.erc20.Approval))
+                  __codec_input_edqy in
               let* α0 :=
                 match __codec_res_edqy with
                 | core.result.Result.Err e =>
@@ -1947,7 +2011,7 @@ Module Impl_parity_scale_codec_codec_Decode_for_erc20_erc20___ink_EventBase.
         let* α0 :=
           (fun  =>
               let* α0 :=
-                core.convert.Into.into
+                (core.convert.Into.into (Self := _))
                   "Could not decode `__ink_EventBase`, variant doesn't exist" in
               Pure (core.result.Result.Err α0)) in
         Return α0 in
@@ -2028,7 +2092,7 @@ Module
   Impl_ink_env_topics_EventTopicsAmount_for_erc20_erc20_____ink_UndefinedAmountOfTopics.
   Definition Self := erc20.erc20._.__ink_UndefinedAmountOfTopics.
   
-  Definition AMOUNT := Pure 0.
+  Definition AMOUNT `{H' : State.Trait} := Pure 0.
   
   Global Instance AssociatedFunction_AMOUNT `{H' : State.Trait} :
     Notation.DoubleColon Self "AMOUNT" := {
@@ -2057,8 +2121,14 @@ Module Impl_ink_env_topics_Topics_for_erc20_erc20___ink_EventBase.
       (builder : ink_env.topics.TopicsBuilder ink_env.topics.state.Uninit E B)
       : M (H := H') ink_env.topics.TopicsBuilderBackend.Output :=
     match self with
-    | Transfer.Build_t event => ink_env.topics.Topics.topics event builder
-    | Approval.Build_t event => ink_env.topics.Topics.topics event builder
+    | Transfer.Build_t event =>
+      (ink_env.topics.Topics.topics (Self := erc20.erc20.Transfer))
+        event
+        builder
+    | Approval.Build_t event =>
+      (ink_env.topics.Topics.topics (Self := erc20.erc20.Approval))
+        event
+        builder
     | _ =>
       let* α0 :=
         format_arguments::["new_const"] (addr_of [ "Event does not exist!" ]) in
@@ -2167,7 +2237,8 @@ Module Impl_parity_scale_codec_encode_like_EncodeLike_for_erc20_erc20_Transfer.
   Definition Self := erc20.erc20.Transfer.
   
   Global Instance I
-    : parity_scale_codec.encode_like.EncodeLike.Trait Self (T := None)
+    : parity_scale_codec.encode_like.EncodeLike.Trait Self
+        (T := parity_scale_codec.encode_like.EncodeLike.Default.T Self)
       := parity_scale_codec.encode_like.EncodeLike.Build_Trait _.
   Global Hint Resolve I : core.
 End Impl_parity_scale_codec_encode_like_EncodeLike_for_erc20_erc20_Transfer.
@@ -2182,7 +2253,9 @@ Module Impl_parity_scale_codec_codec_Decode_for_erc20_erc20_Transfer.
       (__codec_input_edqy : mut_ref __CodecInputEdqy)
       : M (H := H') (core.result.Result Self parity_scale_codec.error.Error) :=
     let* __codec_res_edqy :=
-      parity_scale_codec.codec.Decode.decode __codec_input_edqy in
+      (parity_scale_codec.codec.Decode.decode
+          (Self := (core.option.Option erc20.erc20.AccountId)))
+        __codec_input_edqy in
     let* α0 :=
       match __codec_res_edqy with
       | core.result.Result.Err e =>
@@ -2191,7 +2264,9 @@ Module Impl_parity_scale_codec_codec_Decode_for_erc20_erc20_Transfer.
       | core.result.Result.Ok __codec_res_edqy => Pure __codec_res_edqy
       end in
     let* __codec_res_edqy :=
-      parity_scale_codec.codec.Decode.decode __codec_input_edqy in
+      (parity_scale_codec.codec.Decode.decode
+          (Self := (core.option.Option erc20.erc20.AccountId)))
+        __codec_input_edqy in
     let* α1 :=
       match __codec_res_edqy with
       | core.result.Result.Err e =>
@@ -2200,7 +2275,8 @@ Module Impl_parity_scale_codec_codec_Decode_for_erc20_erc20_Transfer.
       | core.result.Result.Ok __codec_res_edqy => Pure __codec_res_edqy
       end in
     let* __codec_res_edqy :=
-      parity_scale_codec.codec.Decode.decode __codec_input_edqy in
+      (parity_scale_codec.codec.Decode.decode (Self := erc20.erc20.Balance))
+        __codec_input_edqy in
     let* α2 :=
       match __codec_res_edqy with
       | core.result.Result.Err e =>
@@ -2296,7 +2372,8 @@ Module Impl_parity_scale_codec_encode_like_EncodeLike_for_erc20_erc20_Approval.
   Definition Self := erc20.erc20.Approval.
   
   Global Instance I
-    : parity_scale_codec.encode_like.EncodeLike.Trait Self (T := None)
+    : parity_scale_codec.encode_like.EncodeLike.Trait Self
+        (T := parity_scale_codec.encode_like.EncodeLike.Default.T Self)
       := parity_scale_codec.encode_like.EncodeLike.Build_Trait _.
   Global Hint Resolve I : core.
 End Impl_parity_scale_codec_encode_like_EncodeLike_for_erc20_erc20_Approval.
@@ -2311,7 +2388,8 @@ Module Impl_parity_scale_codec_codec_Decode_for_erc20_erc20_Approval.
       (__codec_input_edqy : mut_ref __CodecInputEdqy)
       : M (H := H') (core.result.Result Self parity_scale_codec.error.Error) :=
     let* __codec_res_edqy :=
-      parity_scale_codec.codec.Decode.decode __codec_input_edqy in
+      (parity_scale_codec.codec.Decode.decode (Self := erc20.erc20.AccountId))
+        __codec_input_edqy in
     let* α0 :=
       match __codec_res_edqy with
       | core.result.Result.Err e =>
@@ -2320,7 +2398,8 @@ Module Impl_parity_scale_codec_codec_Decode_for_erc20_erc20_Approval.
       | core.result.Result.Ok __codec_res_edqy => Pure __codec_res_edqy
       end in
     let* __codec_res_edqy :=
-      parity_scale_codec.codec.Decode.decode __codec_input_edqy in
+      (parity_scale_codec.codec.Decode.decode (Self := erc20.erc20.AccountId))
+        __codec_input_edqy in
     let* α1 :=
       match __codec_res_edqy with
       | core.result.Result.Err e =>
@@ -2329,7 +2408,8 @@ Module Impl_parity_scale_codec_codec_Decode_for_erc20_erc20_Approval.
       | core.result.Result.Ok __codec_res_edqy => Pure __codec_res_edqy
       end in
     let* __codec_res_edqy :=
-      parity_scale_codec.codec.Decode.decode __codec_input_edqy in
+      (parity_scale_codec.codec.Decode.decode (Self := erc20.erc20.Balance))
+        __codec_input_edqy in
     let* α2 :=
       match __codec_res_edqy with
       | core.result.Result.Err e =>
@@ -2480,7 +2560,11 @@ Module
   
   Definition Error : Set := ink.reflect.dispatch.ConstructorOutput.Error.
   
-  Definition IS_RESULT `{State.Trait} := Pure ink.reflect.dispatch.ConstructorOutput.IS_RESULT.
+  Definition
+    IS_RESULT
+    `{H' : State.Trait} := Pure
+      (ink.reflect.dispatch.ConstructorOutput.IS_RESULT
+        (Self := (ink.reflect.dispatch.ConstructorOutputValue Self))).
   
   Global Instance AssociatedFunction_IS_RESULT `{H' : State.Trait} :
     Notation.DoubleColon Self "IS_RESULT" := {
@@ -2488,7 +2572,8 @@ Module
   }.
   
   Definition
-    CALLABLE `{State.Trait} := Pure
+    CALLABLE
+    `{H' : State.Trait} := Pure
       (fun __ink_binding_0 => erc20.erc20.Erc20::["new"] __ink_binding_0).
   
   Global Instance AssociatedFunction_CALLABLE `{H' : State.Trait} :
@@ -2496,21 +2581,21 @@ Module
     Notation.double_colon := CALLABLE;
   }.
   
-  Definition PAYABLE := Pure false.
+  Definition PAYABLE `{H' : State.Trait} := Pure false.
   
   Global Instance AssociatedFunction_PAYABLE `{H' : State.Trait} :
     Notation.DoubleColon Self "PAYABLE" := {
     Notation.double_colon := PAYABLE;
   }.
   
-  Definition SELECTOR := Pure [ 155; 174; 157; 94 ].
+  Definition SELECTOR `{H' : State.Trait} := Pure [ 155; 174; 157; 94 ].
   
   Global Instance AssociatedFunction_SELECTOR `{H' : State.Trait} :
     Notation.DoubleColon Self "SELECTOR" := {
     Notation.double_colon := SELECTOR;
   }.
   
-  Definition LABEL := Pure "new".
+  Definition LABEL `{H' : State.Trait} := Pure "new".
   
   Global Instance AssociatedFunction_LABEL `{H' : State.Trait} :
     Notation.DoubleColon Self "LABEL" := {
@@ -2555,7 +2640,8 @@ Module Impl_ink_reflect_dispatch_DispatchableMessageInfo_for_erc20_erc20_Erc20.
   Definition Storage : Set := erc20.erc20.Erc20.
   
   Definition
-    CALLABLE `{State.Trait} := Pure
+    CALLABLE
+    `{H' : State.Trait} := Pure
       (fun storage _ => erc20.erc20.Erc20::["total_supply"] storage).
   
   Global Instance AssociatedFunction_CALLABLE `{H' : State.Trait} :
@@ -2563,28 +2649,28 @@ Module Impl_ink_reflect_dispatch_DispatchableMessageInfo_for_erc20_erc20_Erc20.
     Notation.double_colon := CALLABLE;
   }.
   
-  Definition SELECTOR := Pure [ 219; 99; 117; 168 ].
+  Definition SELECTOR `{H' : State.Trait} := Pure [ 219; 99; 117; 168 ].
   
   Global Instance AssociatedFunction_SELECTOR `{H' : State.Trait} :
     Notation.DoubleColon Self "SELECTOR" := {
     Notation.double_colon := SELECTOR;
   }.
   
-  Definition PAYABLE := Pure false.
+  Definition PAYABLE `{H' : State.Trait} := Pure false.
   
   Global Instance AssociatedFunction_PAYABLE `{H' : State.Trait} :
     Notation.DoubleColon Self "PAYABLE" := {
     Notation.double_colon := PAYABLE;
   }.
   
-  Definition MUTATES := Pure false.
+  Definition MUTATES `{H' : State.Trait} := Pure false.
   
   Global Instance AssociatedFunction_MUTATES `{H' : State.Trait} :
     Notation.DoubleColon Self "MUTATES" := {
     Notation.double_colon := MUTATES;
   }.
   
-  Definition LABEL := Pure "total_supply".
+  Definition LABEL `{H' : State.Trait} := Pure "total_supply".
   
   Global Instance AssociatedFunction_LABEL `{H' : State.Trait} :
     Notation.DoubleColon Self "LABEL" := {
@@ -2625,7 +2711,8 @@ Module Impl_ink_reflect_dispatch_DispatchableMessageInfo_for_erc20_erc20_Erc20.
   Definition Storage : Set := erc20.erc20.Erc20.
   
   Definition
-    CALLABLE `{State.Trait} := Pure
+    CALLABLE
+    `{H' : State.Trait} := Pure
       (fun storage __ink_binding_0 =>
         erc20.erc20.Erc20::["balance_of"] storage __ink_binding_0).
   
@@ -2634,28 +2721,28 @@ Module Impl_ink_reflect_dispatch_DispatchableMessageInfo_for_erc20_erc20_Erc20.
     Notation.double_colon := CALLABLE;
   }.
   
-  Definition SELECTOR := Pure [ 15; 117; 90; 86 ].
+  Definition SELECTOR `{H' : State.Trait} := Pure [ 15; 117; 90; 86 ].
   
   Global Instance AssociatedFunction_SELECTOR `{H' : State.Trait} :
     Notation.DoubleColon Self "SELECTOR" := {
     Notation.double_colon := SELECTOR;
   }.
   
-  Definition PAYABLE := Pure false.
+  Definition PAYABLE `{H' : State.Trait} := Pure false.
   
   Global Instance AssociatedFunction_PAYABLE `{H' : State.Trait} :
     Notation.DoubleColon Self "PAYABLE" := {
     Notation.double_colon := PAYABLE;
   }.
   
-  Definition MUTATES := Pure false.
+  Definition MUTATES `{H' : State.Trait} := Pure false.
   
   Global Instance AssociatedFunction_MUTATES `{H' : State.Trait} :
     Notation.DoubleColon Self "MUTATES" := {
     Notation.double_colon := MUTATES;
   }.
   
-  Definition LABEL := Pure "balance_of".
+  Definition LABEL `{H' : State.Trait} := Pure "balance_of".
   
   Global Instance AssociatedFunction_LABEL `{H' : State.Trait} :
     Notation.DoubleColon Self "LABEL" := {
@@ -2696,7 +2783,8 @@ Module Impl_ink_reflect_dispatch_DispatchableMessageInfo_for_erc20_erc20_Erc20.
   Definition Storage : Set := erc20.erc20.Erc20.
   
   Definition
-    CALLABLE `{State.Trait} := Pure
+    CALLABLE
+    `{H' : State.Trait} := Pure
       (fun storage (__ink_binding_0, __ink_binding_1) =>
         erc20.erc20.Erc20::["allowance"]
           storage
@@ -2708,28 +2796,28 @@ Module Impl_ink_reflect_dispatch_DispatchableMessageInfo_for_erc20_erc20_Erc20.
     Notation.double_colon := CALLABLE;
   }.
   
-  Definition SELECTOR := Pure [ 106; 0; 22; 94 ].
+  Definition SELECTOR `{H' : State.Trait} := Pure [ 106; 0; 22; 94 ].
   
   Global Instance AssociatedFunction_SELECTOR `{H' : State.Trait} :
     Notation.DoubleColon Self "SELECTOR" := {
     Notation.double_colon := SELECTOR;
   }.
   
-  Definition PAYABLE := Pure false.
+  Definition PAYABLE `{H' : State.Trait} := Pure false.
   
   Global Instance AssociatedFunction_PAYABLE `{H' : State.Trait} :
     Notation.DoubleColon Self "PAYABLE" := {
     Notation.double_colon := PAYABLE;
   }.
   
-  Definition MUTATES := Pure false.
+  Definition MUTATES `{H' : State.Trait} := Pure false.
   
   Global Instance AssociatedFunction_MUTATES `{H' : State.Trait} :
     Notation.DoubleColon Self "MUTATES" := {
     Notation.double_colon := MUTATES;
   }.
   
-  Definition LABEL := Pure "allowance".
+  Definition LABEL `{H' : State.Trait} := Pure "allowance".
   
   Global Instance AssociatedFunction_LABEL `{H' : State.Trait} :
     Notation.DoubleColon Self "LABEL" := {
@@ -2770,7 +2858,8 @@ Module Impl_ink_reflect_dispatch_DispatchableMessageInfo_for_erc20_erc20_Erc20.
   Definition Storage : Set := erc20.erc20.Erc20.
   
   Definition
-    CALLABLE `{State.Trait} := Pure
+    CALLABLE
+    `{H' : State.Trait} := Pure
       (fun storage (__ink_binding_0, __ink_binding_1) =>
         erc20.erc20.Erc20::["transfer"]
           storage
@@ -2782,28 +2871,28 @@ Module Impl_ink_reflect_dispatch_DispatchableMessageInfo_for_erc20_erc20_Erc20.
     Notation.double_colon := CALLABLE;
   }.
   
-  Definition SELECTOR := Pure [ 132; 161; 93; 161 ].
+  Definition SELECTOR `{H' : State.Trait} := Pure [ 132; 161; 93; 161 ].
   
   Global Instance AssociatedFunction_SELECTOR `{H' : State.Trait} :
     Notation.DoubleColon Self "SELECTOR" := {
     Notation.double_colon := SELECTOR;
   }.
   
-  Definition PAYABLE := Pure false.
+  Definition PAYABLE `{H' : State.Trait} := Pure false.
   
   Global Instance AssociatedFunction_PAYABLE `{H' : State.Trait} :
     Notation.DoubleColon Self "PAYABLE" := {
     Notation.double_colon := PAYABLE;
   }.
   
-  Definition MUTATES := Pure true.
+  Definition MUTATES `{H' : State.Trait} := Pure true.
   
   Global Instance AssociatedFunction_MUTATES `{H' : State.Trait} :
     Notation.DoubleColon Self "MUTATES" := {
     Notation.double_colon := MUTATES;
   }.
   
-  Definition LABEL := Pure "transfer".
+  Definition LABEL `{H' : State.Trait} := Pure "transfer".
   
   Global Instance AssociatedFunction_LABEL `{H' : State.Trait} :
     Notation.DoubleColon Self "LABEL" := {
@@ -2844,7 +2933,8 @@ Module Impl_ink_reflect_dispatch_DispatchableMessageInfo_for_erc20_erc20_Erc20.
   Definition Storage : Set := erc20.erc20.Erc20.
   
   Definition
-    CALLABLE `{State.Trait} := Pure
+    CALLABLE
+    `{H' : State.Trait} := Pure
       (fun storage (__ink_binding_0, __ink_binding_1) =>
         erc20.erc20.Erc20::["approve"] storage __ink_binding_0 __ink_binding_1).
   
@@ -2853,28 +2943,28 @@ Module Impl_ink_reflect_dispatch_DispatchableMessageInfo_for_erc20_erc20_Erc20.
     Notation.double_colon := CALLABLE;
   }.
   
-  Definition SELECTOR := Pure [ 104; 18; 102; 160 ].
+  Definition SELECTOR `{H' : State.Trait} := Pure [ 104; 18; 102; 160 ].
   
   Global Instance AssociatedFunction_SELECTOR `{H' : State.Trait} :
     Notation.DoubleColon Self "SELECTOR" := {
     Notation.double_colon := SELECTOR;
   }.
   
-  Definition PAYABLE := Pure false.
+  Definition PAYABLE `{H' : State.Trait} := Pure false.
   
   Global Instance AssociatedFunction_PAYABLE `{H' : State.Trait} :
     Notation.DoubleColon Self "PAYABLE" := {
     Notation.double_colon := PAYABLE;
   }.
   
-  Definition MUTATES := Pure true.
+  Definition MUTATES `{H' : State.Trait} := Pure true.
   
   Global Instance AssociatedFunction_MUTATES `{H' : State.Trait} :
     Notation.DoubleColon Self "MUTATES" := {
     Notation.double_colon := MUTATES;
   }.
   
-  Definition LABEL := Pure "approve".
+  Definition LABEL `{H' : State.Trait} := Pure "approve".
   
   Global Instance AssociatedFunction_LABEL `{H' : State.Trait} :
     Notation.DoubleColon Self "LABEL" := {
@@ -2916,7 +3006,8 @@ Module Impl_ink_reflect_dispatch_DispatchableMessageInfo_for_erc20_erc20_Erc20.
   Definition Storage : Set := erc20.erc20.Erc20.
   
   Definition
-    CALLABLE `{State.Trait} := Pure
+    CALLABLE
+    `{H' : State.Trait} := Pure
       (fun storage (__ink_binding_0, __ink_binding_1, __ink_binding_2) =>
         erc20.erc20.Erc20::["transfer_from"]
           storage
@@ -2929,28 +3020,28 @@ Module Impl_ink_reflect_dispatch_DispatchableMessageInfo_for_erc20_erc20_Erc20.
     Notation.double_colon := CALLABLE;
   }.
   
-  Definition SELECTOR := Pure [ 11; 57; 111; 24 ].
+  Definition SELECTOR `{H' : State.Trait} := Pure [ 11; 57; 111; 24 ].
   
   Global Instance AssociatedFunction_SELECTOR `{H' : State.Trait} :
     Notation.DoubleColon Self "SELECTOR" := {
     Notation.double_colon := SELECTOR;
   }.
   
-  Definition PAYABLE := Pure false.
+  Definition PAYABLE `{H' : State.Trait} := Pure false.
   
   Global Instance AssociatedFunction_PAYABLE `{H' : State.Trait} :
     Notation.DoubleColon Self "PAYABLE" := {
     Notation.double_colon := PAYABLE;
   }.
   
-  Definition MUTATES := Pure true.
+  Definition MUTATES `{H' : State.Trait} := Pure true.
   
   Global Instance AssociatedFunction_MUTATES `{H' : State.Trait} :
     Notation.DoubleColon Self "MUTATES" := {
     Notation.double_colon := MUTATES;
   }.
   
-  Definition LABEL := Pure "transfer_from".
+  Definition LABEL `{H' : State.Trait} := Pure "transfer_from".
   
   Global Instance AssociatedFunction_LABEL `{H' : State.Trait} :
     Notation.DoubleColon Self "LABEL" := {
@@ -2999,7 +3090,10 @@ Module
       :
         M (H := H')
           (core.result.Result Self ink.reflect.dispatch.DispatchError) :=
-    let* α0 := parity_scale_codec.codec.Decode.decode input in
+    let* α0 :=
+      (parity_scale_codec.codec.Decode.decode
+          (Self := (list Root.core.primitive.u8)))
+        input in
     let* α1 :=
       α0.["map_err"]
         (fun _ => Pure ink.reflect.dispatch.DispatchError.InvalidSelector) in
@@ -3013,7 +3107,10 @@ Module
       end in
     match α3 with
     | erc20.erc20._.decode_dispatch.CONSTRUCTOR_0 =>
-      let* α0 := parity_scale_codec.codec.Decode.decode input in
+      let* α0 :=
+        (parity_scale_codec.codec.Decode.decode
+            (Self := ink.reflect.dispatch.DispatchableConstructorInfo.Input))
+          input in
       let* α1 :=
         α0.["map_err"]
           (fun _ =>
@@ -3049,7 +3146,10 @@ End
   Impl_ink_reflect_dispatch_DecodeDispatch_for_erc20_erc20_____ink_ConstructorDecoder.
 
 Definition CONSTRUCTOR_0 `{H' : State.Trait} : list Root.core.primitive.u8 :=
-  run (Pure ink.reflect.dispatch.DispatchableConstructorInfo.SELECTOR).
+  run
+    (Pure
+      (ink.reflect.dispatch.DispatchableConstructorInfo.SELECTOR
+        (Self := erc20.erc20.Erc20))).
 
 Module
   Impl_parity_scale_codec_codec_Decode_for_erc20_erc20_____ink_ConstructorDecoder.
@@ -3061,7 +3161,9 @@ Module
       `{parity_scale_codec.codec.Input.Trait I}
       (input : mut_ref I)
       : M (H := H') (core.result.Result Self parity_scale_codec.error.Error) :=
-    let* α0 := ink.reflect.dispatch.DecodeDispatch.decode_dispatch input in
+    let* α0 :=
+      (ink.reflect.dispatch.DecodeDispatch.decode_dispatch (Self := Self))
+        input in
     α0.["map_err"] core.convert.Into.into.
   
   Global Instance AssociatedFunction_decode `{H' : State.Trait} :
@@ -3091,10 +3193,12 @@ Module
       let* _ :=
         let constructor_0 := false in
         let constructor_0 :=
-          ink.reflect.dispatch.DispatchableConstructorInfo.PAYABLE in
+          ink.reflect.dispatch.DispatchableConstructorInfo.PAYABLE
+            (Self := erc20.erc20.Erc20) in
         let* α0 := false.["or"] constructor_0 in
         let* α1 :=
-          ink.reflect.dispatch.DispatchableConstructorInfo.PAYABLE.["not"] in
+          (ink.reflect.dispatch.DispatchableConstructorInfo.PAYABLE
+              (Self := erc20.erc20.Erc20)).["not"] in
         let* α2 := α0.["andb"] α1 in
         if (α2 : bool) then
           let* _ :=
@@ -3110,11 +3214,16 @@ Module
         else
           Pure tt in
       let* result :=
-        ink.reflect.dispatch.DispatchableConstructorInfo.CALLABLE input in
+        (ink.reflect.dispatch.DispatchableConstructorInfo.CALLABLE
+            (Self := erc20.erc20.Erc20))
+          input in
       let* output_value :=
         ink.reflect.dispatch.ConstructorOutputValue::["new"] result in
       let* output_result :=
-        ink.reflect.dispatch.ConstructorOutput.as_result
+        (ink.reflect.dispatch.ConstructorOutput.as_result
+            (Self :=
+              (ink.reflect.dispatch.ConstructorOutputValue
+                ink.reflect.dispatch.DispatchableConstructorInfo.Output)))
           (addr_of output_value) in
       let* _ :=
         let* α0 := output_result.["as_ref"] in
@@ -3122,7 +3231,9 @@ Module
         | core.result.Result.Ok contract =>
           let* _ :=
             ink_env.api.set_contract_storage
-              (addr_of ink_storage_traits.storage.StorageKey.KEY)
+              (addr_of
+                (ink_storage_traits.storage.StorageKey.KEY
+                  (Self := erc20.erc20.Erc20)))
               contract in
           Pure tt
         | _ => Pure tt
@@ -3189,7 +3300,10 @@ Module
       :
         M (H := H')
           (core.result.Result Self ink.reflect.dispatch.DispatchError) :=
-    let* α0 := parity_scale_codec.codec.Decode.decode input in
+    let* α0 :=
+      (parity_scale_codec.codec.Decode.decode
+          (Self := (list Root.core.primitive.u8)))
+        input in
     let* α1 :=
       α0.["map_err"]
         (fun _ => Pure ink.reflect.dispatch.DispatchError.InvalidSelector) in
@@ -3203,7 +3317,10 @@ Module
       end in
     match α3 with
     | erc20.erc20._.decode_dispatch.MESSAGE_0 =>
-      let* α0 := parity_scale_codec.codec.Decode.decode input in
+      let* α0 :=
+        (parity_scale_codec.codec.Decode.decode
+            (Self := ink.reflect.dispatch.DispatchableMessageInfo.Input))
+          input in
       let* α1 :=
         α0.["map_err"]
           (fun _ =>
@@ -3219,7 +3336,10 @@ Module
       let* α4 := Self::["Message0"] α3 in
       Pure (core.result.Result.Ok α4)
     | erc20.erc20._.decode_dispatch.MESSAGE_1 =>
-      let* α0 := parity_scale_codec.codec.Decode.decode input in
+      let* α0 :=
+        (parity_scale_codec.codec.Decode.decode
+            (Self := ink.reflect.dispatch.DispatchableMessageInfo.Input))
+          input in
       let* α1 :=
         α0.["map_err"]
           (fun _ =>
@@ -3235,7 +3355,10 @@ Module
       let* α4 := Self::["Message1"] α3 in
       Pure (core.result.Result.Ok α4)
     | erc20.erc20._.decode_dispatch.MESSAGE_2 =>
-      let* α0 := parity_scale_codec.codec.Decode.decode input in
+      let* α0 :=
+        (parity_scale_codec.codec.Decode.decode
+            (Self := ink.reflect.dispatch.DispatchableMessageInfo.Input))
+          input in
       let* α1 :=
         α0.["map_err"]
           (fun _ =>
@@ -3251,7 +3374,10 @@ Module
       let* α4 := Self::["Message2"] α3 in
       Pure (core.result.Result.Ok α4)
     | erc20.erc20._.decode_dispatch.MESSAGE_3 =>
-      let* α0 := parity_scale_codec.codec.Decode.decode input in
+      let* α0 :=
+        (parity_scale_codec.codec.Decode.decode
+            (Self := ink.reflect.dispatch.DispatchableMessageInfo.Input))
+          input in
       let* α1 :=
         α0.["map_err"]
           (fun _ =>
@@ -3267,7 +3393,10 @@ Module
       let* α4 := Self::["Message3"] α3 in
       Pure (core.result.Result.Ok α4)
     | erc20.erc20._.decode_dispatch.MESSAGE_4 =>
-      let* α0 := parity_scale_codec.codec.Decode.decode input in
+      let* α0 :=
+        (parity_scale_codec.codec.Decode.decode
+            (Self := ink.reflect.dispatch.DispatchableMessageInfo.Input))
+          input in
       let* α1 :=
         α0.["map_err"]
           (fun _ =>
@@ -3283,7 +3412,10 @@ Module
       let* α4 := Self::["Message4"] α3 in
       Pure (core.result.Result.Ok α4)
     | erc20.erc20._.decode_dispatch.MESSAGE_5 =>
-      let* α0 := parity_scale_codec.codec.Decode.decode input in
+      let* α0 :=
+        (parity_scale_codec.codec.Decode.decode
+            (Self := ink.reflect.dispatch.DispatchableMessageInfo.Input))
+          input in
       let* α1 :=
         α0.["map_err"]
           (fun _ =>
@@ -3319,22 +3451,40 @@ End
   Impl_ink_reflect_dispatch_DecodeDispatch_for_erc20_erc20_____ink_MessageDecoder.
 
 Definition MESSAGE_0 `{H' : State.Trait} : list Root.core.primitive.u8 :=
-  run (Pure ink.reflect.dispatch.DispatchableMessageInfo.SELECTOR).
+  run
+    (Pure
+      (ink.reflect.dispatch.DispatchableMessageInfo.SELECTOR
+        (Self := erc20.erc20.Erc20))).
 
 Definition MESSAGE_1 `{H' : State.Trait} : list Root.core.primitive.u8 :=
-  run (Pure ink.reflect.dispatch.DispatchableMessageInfo.SELECTOR).
+  run
+    (Pure
+      (ink.reflect.dispatch.DispatchableMessageInfo.SELECTOR
+        (Self := erc20.erc20.Erc20))).
 
 Definition MESSAGE_2 `{H' : State.Trait} : list Root.core.primitive.u8 :=
-  run (Pure ink.reflect.dispatch.DispatchableMessageInfo.SELECTOR).
+  run
+    (Pure
+      (ink.reflect.dispatch.DispatchableMessageInfo.SELECTOR
+        (Self := erc20.erc20.Erc20))).
 
 Definition MESSAGE_3 `{H' : State.Trait} : list Root.core.primitive.u8 :=
-  run (Pure ink.reflect.dispatch.DispatchableMessageInfo.SELECTOR).
+  run
+    (Pure
+      (ink.reflect.dispatch.DispatchableMessageInfo.SELECTOR
+        (Self := erc20.erc20.Erc20))).
 
 Definition MESSAGE_4 `{H' : State.Trait} : list Root.core.primitive.u8 :=
-  run (Pure ink.reflect.dispatch.DispatchableMessageInfo.SELECTOR).
+  run
+    (Pure
+      (ink.reflect.dispatch.DispatchableMessageInfo.SELECTOR
+        (Self := erc20.erc20.Erc20))).
 
 Definition MESSAGE_5 `{H' : State.Trait} : list Root.core.primitive.u8 :=
-  run (Pure ink.reflect.dispatch.DispatchableMessageInfo.SELECTOR).
+  run
+    (Pure
+      (ink.reflect.dispatch.DispatchableMessageInfo.SELECTOR
+        (Self := erc20.erc20.Erc20))).
 
 Module
   Impl_parity_scale_codec_codec_Decode_for_erc20_erc20_____ink_MessageDecoder.
@@ -3346,7 +3496,9 @@ Module
       `{parity_scale_codec.codec.Input.Trait I}
       (input : mut_ref I)
       : M (H := H') (core.result.Result Self parity_scale_codec.error.Error) :=
-    let* α0 := ink.reflect.dispatch.DecodeDispatch.decode_dispatch input in
+    let* α0 :=
+      (ink.reflect.dispatch.DecodeDispatch.decode_dispatch (Self := Self))
+        input in
     α0.["map_err"] core.convert.Into.into.
   
   Global Instance AssociatedFunction_decode `{H' : State.Trait} :
@@ -3368,7 +3520,9 @@ Definition push_contract
   if (mutates : bool) then
     let* _ :=
       ink_env.api.set_contract_storage
-        (addr_of ink_storage_traits.storage.StorageKey.KEY)
+        (addr_of
+          (ink_storage_traits.storage.StorageKey.KEY
+            (Self := erc20.erc20.Erc20)))
         (addr_of contract) in
     Pure tt
   else
@@ -3384,7 +3538,8 @@ Module
       :
         M (H := H')
           (core.result.Result unit ink.reflect.dispatch.DispatchError) :=
-    let key := ink_storage_traits.storage.StorageKey.KEY in
+    let key :=
+      ink_storage_traits.storage.StorageKey.KEY (Self := erc20.erc20.Erc20) in
     let* contract :=
       let* α0 := ink_env.api.get_contract_storage (addr_of key) in
       let* α1 :=
@@ -3408,30 +3563,37 @@ Module
         let* _ :=
           let message_0 := false in
           let message_0 :=
-            ink.reflect.dispatch.DispatchableMessageInfo.PAYABLE in
+            ink.reflect.dispatch.DispatchableMessageInfo.PAYABLE
+              (Self := erc20.erc20.Erc20) in
           let* α0 := false.["or"] message_0 in
           let message_1 := false in
           let message_1 :=
-            ink.reflect.dispatch.DispatchableMessageInfo.PAYABLE in
+            ink.reflect.dispatch.DispatchableMessageInfo.PAYABLE
+              (Self := erc20.erc20.Erc20) in
           let* α1 := α0.["or"] message_1 in
           let message_2 := false in
           let message_2 :=
-            ink.reflect.dispatch.DispatchableMessageInfo.PAYABLE in
+            ink.reflect.dispatch.DispatchableMessageInfo.PAYABLE
+              (Self := erc20.erc20.Erc20) in
           let* α2 := α1.["or"] message_2 in
           let message_3 := false in
           let message_3 :=
-            ink.reflect.dispatch.DispatchableMessageInfo.PAYABLE in
+            ink.reflect.dispatch.DispatchableMessageInfo.PAYABLE
+              (Self := erc20.erc20.Erc20) in
           let* α3 := α2.["or"] message_3 in
           let message_4 := false in
           let message_4 :=
-            ink.reflect.dispatch.DispatchableMessageInfo.PAYABLE in
+            ink.reflect.dispatch.DispatchableMessageInfo.PAYABLE
+              (Self := erc20.erc20.Erc20) in
           let* α4 := α3.["or"] message_4 in
           let message_5 := false in
           let message_5 :=
-            ink.reflect.dispatch.DispatchableMessageInfo.PAYABLE in
+            ink.reflect.dispatch.DispatchableMessageInfo.PAYABLE
+              (Self := erc20.erc20.Erc20) in
           let* α0 := α4.["or"] message_5 in
           let* α1 :=
-            ink.reflect.dispatch.DispatchableMessageInfo.PAYABLE.["not"] in
+            (ink.reflect.dispatch.DispatchableMessageInfo.PAYABLE
+                (Self := erc20.erc20.Erc20)).["not"] in
           let* α2 := α0.["andb"] α1 in
           if (α2 : bool) then
             let* _ :=
@@ -3447,7 +3609,8 @@ Module
           else
             Pure tt in
         let* result :=
-          ink.reflect.dispatch.DispatchableMessageInfo.CALLABLE
+          (ink.reflect.dispatch.DispatchableMessageInfo.CALLABLE
+              (Self := erc20.erc20.Erc20))
             (addr_of contract)
             input in
         let* is_reverted :=
@@ -3462,7 +3625,8 @@ Module
             let* _ :=
               erc20.erc20._.push_contract
                 contract
-                ink.reflect.dispatch.DispatchableMessageInfo.MUTATES in
+                (ink.reflect.dispatch.DispatchableMessageInfo.MUTATES
+                  (Self := erc20.erc20.Erc20)) in
             Pure tt
           else
             Pure tt in
@@ -3475,30 +3639,37 @@ Module
         let* _ :=
           let message_0 := false in
           let message_0 :=
-            ink.reflect.dispatch.DispatchableMessageInfo.PAYABLE in
+            ink.reflect.dispatch.DispatchableMessageInfo.PAYABLE
+              (Self := erc20.erc20.Erc20) in
           let* α0 := false.["or"] message_0 in
           let message_1 := false in
           let message_1 :=
-            ink.reflect.dispatch.DispatchableMessageInfo.PAYABLE in
+            ink.reflect.dispatch.DispatchableMessageInfo.PAYABLE
+              (Self := erc20.erc20.Erc20) in
           let* α1 := α0.["or"] message_1 in
           let message_2 := false in
           let message_2 :=
-            ink.reflect.dispatch.DispatchableMessageInfo.PAYABLE in
+            ink.reflect.dispatch.DispatchableMessageInfo.PAYABLE
+              (Self := erc20.erc20.Erc20) in
           let* α2 := α1.["or"] message_2 in
           let message_3 := false in
           let message_3 :=
-            ink.reflect.dispatch.DispatchableMessageInfo.PAYABLE in
+            ink.reflect.dispatch.DispatchableMessageInfo.PAYABLE
+              (Self := erc20.erc20.Erc20) in
           let* α3 := α2.["or"] message_3 in
           let message_4 := false in
           let message_4 :=
-            ink.reflect.dispatch.DispatchableMessageInfo.PAYABLE in
+            ink.reflect.dispatch.DispatchableMessageInfo.PAYABLE
+              (Self := erc20.erc20.Erc20) in
           let* α4 := α3.["or"] message_4 in
           let message_5 := false in
           let message_5 :=
-            ink.reflect.dispatch.DispatchableMessageInfo.PAYABLE in
+            ink.reflect.dispatch.DispatchableMessageInfo.PAYABLE
+              (Self := erc20.erc20.Erc20) in
           let* α0 := α4.["or"] message_5 in
           let* α1 :=
-            ink.reflect.dispatch.DispatchableMessageInfo.PAYABLE.["not"] in
+            (ink.reflect.dispatch.DispatchableMessageInfo.PAYABLE
+                (Self := erc20.erc20.Erc20)).["not"] in
           let* α2 := α0.["andb"] α1 in
           if (α2 : bool) then
             let* _ :=
@@ -3514,7 +3685,8 @@ Module
           else
             Pure tt in
         let* result :=
-          ink.reflect.dispatch.DispatchableMessageInfo.CALLABLE
+          (ink.reflect.dispatch.DispatchableMessageInfo.CALLABLE
+              (Self := erc20.erc20.Erc20))
             (addr_of contract)
             input in
         let* is_reverted :=
@@ -3529,7 +3701,8 @@ Module
             let* _ :=
               erc20.erc20._.push_contract
                 contract
-                ink.reflect.dispatch.DispatchableMessageInfo.MUTATES in
+                (ink.reflect.dispatch.DispatchableMessageInfo.MUTATES
+                  (Self := erc20.erc20.Erc20)) in
             Pure tt
           else
             Pure tt in
@@ -3542,30 +3715,37 @@ Module
         let* _ :=
           let message_0 := false in
           let message_0 :=
-            ink.reflect.dispatch.DispatchableMessageInfo.PAYABLE in
+            ink.reflect.dispatch.DispatchableMessageInfo.PAYABLE
+              (Self := erc20.erc20.Erc20) in
           let* α0 := false.["or"] message_0 in
           let message_1 := false in
           let message_1 :=
-            ink.reflect.dispatch.DispatchableMessageInfo.PAYABLE in
+            ink.reflect.dispatch.DispatchableMessageInfo.PAYABLE
+              (Self := erc20.erc20.Erc20) in
           let* α1 := α0.["or"] message_1 in
           let message_2 := false in
           let message_2 :=
-            ink.reflect.dispatch.DispatchableMessageInfo.PAYABLE in
+            ink.reflect.dispatch.DispatchableMessageInfo.PAYABLE
+              (Self := erc20.erc20.Erc20) in
           let* α2 := α1.["or"] message_2 in
           let message_3 := false in
           let message_3 :=
-            ink.reflect.dispatch.DispatchableMessageInfo.PAYABLE in
+            ink.reflect.dispatch.DispatchableMessageInfo.PAYABLE
+              (Self := erc20.erc20.Erc20) in
           let* α3 := α2.["or"] message_3 in
           let message_4 := false in
           let message_4 :=
-            ink.reflect.dispatch.DispatchableMessageInfo.PAYABLE in
+            ink.reflect.dispatch.DispatchableMessageInfo.PAYABLE
+              (Self := erc20.erc20.Erc20) in
           let* α4 := α3.["or"] message_4 in
           let message_5 := false in
           let message_5 :=
-            ink.reflect.dispatch.DispatchableMessageInfo.PAYABLE in
+            ink.reflect.dispatch.DispatchableMessageInfo.PAYABLE
+              (Self := erc20.erc20.Erc20) in
           let* α0 := α4.["or"] message_5 in
           let* α1 :=
-            ink.reflect.dispatch.DispatchableMessageInfo.PAYABLE.["not"] in
+            (ink.reflect.dispatch.DispatchableMessageInfo.PAYABLE
+                (Self := erc20.erc20.Erc20)).["not"] in
           let* α2 := α0.["andb"] α1 in
           if (α2 : bool) then
             let* _ :=
@@ -3581,7 +3761,8 @@ Module
           else
             Pure tt in
         let* result :=
-          ink.reflect.dispatch.DispatchableMessageInfo.CALLABLE
+          (ink.reflect.dispatch.DispatchableMessageInfo.CALLABLE
+              (Self := erc20.erc20.Erc20))
             (addr_of contract)
             input in
         let* is_reverted :=
@@ -3596,7 +3777,8 @@ Module
             let* _ :=
               erc20.erc20._.push_contract
                 contract
-                ink.reflect.dispatch.DispatchableMessageInfo.MUTATES in
+                (ink.reflect.dispatch.DispatchableMessageInfo.MUTATES
+                  (Self := erc20.erc20.Erc20)) in
             Pure tt
           else
             Pure tt in
@@ -3609,30 +3791,37 @@ Module
         let* _ :=
           let message_0 := false in
           let message_0 :=
-            ink.reflect.dispatch.DispatchableMessageInfo.PAYABLE in
+            ink.reflect.dispatch.DispatchableMessageInfo.PAYABLE
+              (Self := erc20.erc20.Erc20) in
           let* α0 := false.["or"] message_0 in
           let message_1 := false in
           let message_1 :=
-            ink.reflect.dispatch.DispatchableMessageInfo.PAYABLE in
+            ink.reflect.dispatch.DispatchableMessageInfo.PAYABLE
+              (Self := erc20.erc20.Erc20) in
           let* α1 := α0.["or"] message_1 in
           let message_2 := false in
           let message_2 :=
-            ink.reflect.dispatch.DispatchableMessageInfo.PAYABLE in
+            ink.reflect.dispatch.DispatchableMessageInfo.PAYABLE
+              (Self := erc20.erc20.Erc20) in
           let* α2 := α1.["or"] message_2 in
           let message_3 := false in
           let message_3 :=
-            ink.reflect.dispatch.DispatchableMessageInfo.PAYABLE in
+            ink.reflect.dispatch.DispatchableMessageInfo.PAYABLE
+              (Self := erc20.erc20.Erc20) in
           let* α3 := α2.["or"] message_3 in
           let message_4 := false in
           let message_4 :=
-            ink.reflect.dispatch.DispatchableMessageInfo.PAYABLE in
+            ink.reflect.dispatch.DispatchableMessageInfo.PAYABLE
+              (Self := erc20.erc20.Erc20) in
           let* α4 := α3.["or"] message_4 in
           let message_5 := false in
           let message_5 :=
-            ink.reflect.dispatch.DispatchableMessageInfo.PAYABLE in
+            ink.reflect.dispatch.DispatchableMessageInfo.PAYABLE
+              (Self := erc20.erc20.Erc20) in
           let* α0 := α4.["or"] message_5 in
           let* α1 :=
-            ink.reflect.dispatch.DispatchableMessageInfo.PAYABLE.["not"] in
+            (ink.reflect.dispatch.DispatchableMessageInfo.PAYABLE
+                (Self := erc20.erc20.Erc20)).["not"] in
           let* α2 := α0.["andb"] α1 in
           if (α2 : bool) then
             let* _ :=
@@ -3648,7 +3837,8 @@ Module
           else
             Pure tt in
         let* result :=
-          ink.reflect.dispatch.DispatchableMessageInfo.CALLABLE
+          (ink.reflect.dispatch.DispatchableMessageInfo.CALLABLE
+              (Self := erc20.erc20.Erc20))
             (addr_of contract)
             input in
         let* is_reverted :=
@@ -3663,7 +3853,8 @@ Module
             let* _ :=
               erc20.erc20._.push_contract
                 contract
-                ink.reflect.dispatch.DispatchableMessageInfo.MUTATES in
+                (ink.reflect.dispatch.DispatchableMessageInfo.MUTATES
+                  (Self := erc20.erc20.Erc20)) in
             Pure tt
           else
             Pure tt in
@@ -3676,30 +3867,37 @@ Module
         let* _ :=
           let message_0 := false in
           let message_0 :=
-            ink.reflect.dispatch.DispatchableMessageInfo.PAYABLE in
+            ink.reflect.dispatch.DispatchableMessageInfo.PAYABLE
+              (Self := erc20.erc20.Erc20) in
           let* α0 := false.["or"] message_0 in
           let message_1 := false in
           let message_1 :=
-            ink.reflect.dispatch.DispatchableMessageInfo.PAYABLE in
+            ink.reflect.dispatch.DispatchableMessageInfo.PAYABLE
+              (Self := erc20.erc20.Erc20) in
           let* α1 := α0.["or"] message_1 in
           let message_2 := false in
           let message_2 :=
-            ink.reflect.dispatch.DispatchableMessageInfo.PAYABLE in
+            ink.reflect.dispatch.DispatchableMessageInfo.PAYABLE
+              (Self := erc20.erc20.Erc20) in
           let* α2 := α1.["or"] message_2 in
           let message_3 := false in
           let message_3 :=
-            ink.reflect.dispatch.DispatchableMessageInfo.PAYABLE in
+            ink.reflect.dispatch.DispatchableMessageInfo.PAYABLE
+              (Self := erc20.erc20.Erc20) in
           let* α3 := α2.["or"] message_3 in
           let message_4 := false in
           let message_4 :=
-            ink.reflect.dispatch.DispatchableMessageInfo.PAYABLE in
+            ink.reflect.dispatch.DispatchableMessageInfo.PAYABLE
+              (Self := erc20.erc20.Erc20) in
           let* α4 := α3.["or"] message_4 in
           let message_5 := false in
           let message_5 :=
-            ink.reflect.dispatch.DispatchableMessageInfo.PAYABLE in
+            ink.reflect.dispatch.DispatchableMessageInfo.PAYABLE
+              (Self := erc20.erc20.Erc20) in
           let* α0 := α4.["or"] message_5 in
           let* α1 :=
-            ink.reflect.dispatch.DispatchableMessageInfo.PAYABLE.["not"] in
+            (ink.reflect.dispatch.DispatchableMessageInfo.PAYABLE
+                (Self := erc20.erc20.Erc20)).["not"] in
           let* α2 := α0.["andb"] α1 in
           if (α2 : bool) then
             let* _ :=
@@ -3715,7 +3913,8 @@ Module
           else
             Pure tt in
         let* result :=
-          ink.reflect.dispatch.DispatchableMessageInfo.CALLABLE
+          (ink.reflect.dispatch.DispatchableMessageInfo.CALLABLE
+              (Self := erc20.erc20.Erc20))
             (addr_of contract)
             input in
         let* is_reverted :=
@@ -3730,7 +3929,8 @@ Module
             let* _ :=
               erc20.erc20._.push_contract
                 contract
-                ink.reflect.dispatch.DispatchableMessageInfo.MUTATES in
+                (ink.reflect.dispatch.DispatchableMessageInfo.MUTATES
+                  (Self := erc20.erc20.Erc20)) in
             Pure tt
           else
             Pure tt in
@@ -3743,30 +3943,37 @@ Module
         let* _ :=
           let message_0 := false in
           let message_0 :=
-            ink.reflect.dispatch.DispatchableMessageInfo.PAYABLE in
+            ink.reflect.dispatch.DispatchableMessageInfo.PAYABLE
+              (Self := erc20.erc20.Erc20) in
           let* α0 := false.["or"] message_0 in
           let message_1 := false in
           let message_1 :=
-            ink.reflect.dispatch.DispatchableMessageInfo.PAYABLE in
+            ink.reflect.dispatch.DispatchableMessageInfo.PAYABLE
+              (Self := erc20.erc20.Erc20) in
           let* α1 := α0.["or"] message_1 in
           let message_2 := false in
           let message_2 :=
-            ink.reflect.dispatch.DispatchableMessageInfo.PAYABLE in
+            ink.reflect.dispatch.DispatchableMessageInfo.PAYABLE
+              (Self := erc20.erc20.Erc20) in
           let* α2 := α1.["or"] message_2 in
           let message_3 := false in
           let message_3 :=
-            ink.reflect.dispatch.DispatchableMessageInfo.PAYABLE in
+            ink.reflect.dispatch.DispatchableMessageInfo.PAYABLE
+              (Self := erc20.erc20.Erc20) in
           let* α3 := α2.["or"] message_3 in
           let message_4 := false in
           let message_4 :=
-            ink.reflect.dispatch.DispatchableMessageInfo.PAYABLE in
+            ink.reflect.dispatch.DispatchableMessageInfo.PAYABLE
+              (Self := erc20.erc20.Erc20) in
           let* α4 := α3.["or"] message_4 in
           let message_5 := false in
           let message_5 :=
-            ink.reflect.dispatch.DispatchableMessageInfo.PAYABLE in
+            ink.reflect.dispatch.DispatchableMessageInfo.PAYABLE
+              (Self := erc20.erc20.Erc20) in
           let* α0 := α4.["or"] message_5 in
           let* α1 :=
-            ink.reflect.dispatch.DispatchableMessageInfo.PAYABLE.["not"] in
+            (ink.reflect.dispatch.DispatchableMessageInfo.PAYABLE
+                (Self := erc20.erc20.Erc20)).["not"] in
           let* α2 := α0.["andb"] α1 in
           if (α2 : bool) then
             let* _ :=
@@ -3782,7 +3989,8 @@ Module
           else
             Pure tt in
         let* result :=
-          ink.reflect.dispatch.DispatchableMessageInfo.CALLABLE
+          (ink.reflect.dispatch.DispatchableMessageInfo.CALLABLE
+              (Self := erc20.erc20.Erc20))
             (addr_of contract)
             input in
         let* is_reverted :=
@@ -3797,7 +4005,8 @@ Module
             let* _ :=
               erc20.erc20._.push_contract
                 contract
-                ink.reflect.dispatch.DispatchableMessageInfo.MUTATES in
+                (ink.reflect.dispatch.DispatchableMessageInfo.MUTATES
+                  (Self := erc20.erc20.Erc20)) in
             Pure tt
           else
             Pure tt in
@@ -4167,7 +4376,8 @@ Module
   Definition Self := erc20.erc20._.CallBuilder.
   
   Global Instance I
-    : parity_scale_codec.encode_like.EncodeLike.Trait Self (T := None)
+    : parity_scale_codec.encode_like.EncodeLike.Trait Self
+        (T := parity_scale_codec.encode_like.EncodeLike.Default.T Self)
       := parity_scale_codec.encode_like.EncodeLike.Build_Trait _.
   Global Hint Resolve I : core.
 End
@@ -4183,7 +4393,8 @@ Module Impl_parity_scale_codec_codec_Decode_for_erc20_erc20___CallBuilder.
       (__codec_input_edqy : mut_ref __CodecInputEdqy)
       : M (H := H') (core.result.Result Self parity_scale_codec.error.Error) :=
     let* __codec_res_edqy :=
-      parity_scale_codec.codec.Decode.decode __codec_input_edqy in
+      (parity_scale_codec.codec.Decode.decode (Self := erc20.erc20.AccountId))
+        __codec_input_edqy in
     let* α0 :=
       match __codec_res_edqy with
       | core.result.Result.Err e =>
@@ -4259,7 +4470,10 @@ Module Impl_parity_scale_codec_codec_Decode_for_erc20_erc20___CallBuilder.
         Pure (addr_of α2) in
       let* _ :=
         let* α0 :=
-          parity_scale_codec.codec.Decode.decode_into __codec_input_edqy dst_ in
+          (parity_scale_codec.codec.Decode.decode_into
+              (Self := erc20.erc20.AccountId))
+            __codec_input_edqy
+            dst_ in
         let* α1 := α0.["branch"] in
         match α1 with
         | LanguageItem.Break residual =>
@@ -4328,7 +4542,9 @@ Module Impl_core_cmp_PartialEq_for_erc20_erc20___CallBuilder.
     Notation.dot := eq;
   }.
   
-  Global Instance I : core.cmp.PartialEq.Trait Self (Rhs := None) := {
+  Global Instance I
+    : core.cmp.PartialEq.Trait Self (Rhs := core.cmp.PartialEq.Default.Rhs Self)
+      := {
     core.cmp.PartialEq.eq `{H' : State.Trait} := eq;
   }.
   Global Hint Resolve I : core.
@@ -4432,7 +4648,10 @@ Module
       `{H' : State.Trait}
       (__key : ref ink_primitives.key.Key)
       : M (H := H') ink_metadata.layout.Layout :=
-    let* α0 := ink_storage_traits.layout.StorageLayout.layout __key in
+    let* α0 :=
+      (ink_storage_traits.layout.StorageLayout.layout
+          (Self := erc20.erc20.AccountId))
+        __key in
     let* α1 := ink_metadata.layout.FieldLayout::["new"] "account_id" α0 in
     let* α2 := ink_metadata.layout.StructLayout::["new"] "CallBuilder" [ α1 ] in
     Pure (ink_metadata.layout.Layout.Struct α2).
@@ -4508,7 +4727,8 @@ Module Impl_ink_contract_ref_ToAccountId_for_erc20_erc20___CallBuilder.
       `{H' : State.Trait}
       (self : ref Self)
       : M (H := H') erc20.erc20.AccountId :=
-    core.clone.Clone.clone (addr_of self.["account_id"]).
+    (core.clone.Clone.clone (Self := erc20.erc20.AccountId))
+      (addr_of self.["account_id"]).
   
   Global Instance Method_to_account_id `{H' : State.Trait} :
     Notation.Dot "to_account_id" := {
@@ -4895,7 +5115,8 @@ Module Impl_parity_scale_codec_encode_like_EncodeLike_for_erc20_erc20_Erc20Ref.
   Definition Self := erc20.erc20.Erc20Ref.
   
   Global Instance I
-    : parity_scale_codec.encode_like.EncodeLike.Trait Self (T := None)
+    : parity_scale_codec.encode_like.EncodeLike.Trait Self
+        (T := parity_scale_codec.encode_like.EncodeLike.Default.T Self)
       := parity_scale_codec.encode_like.EncodeLike.Build_Trait _.
   Global Hint Resolve I : core.
 End Impl_parity_scale_codec_encode_like_EncodeLike_for_erc20_erc20_Erc20Ref.
@@ -4910,7 +5131,9 @@ Module Impl_parity_scale_codec_codec_Decode_for_erc20_erc20_Erc20Ref.
       (__codec_input_edqy : mut_ref __CodecInputEdqy)
       : M (H := H') (core.result.Result Self parity_scale_codec.error.Error) :=
     let* __codec_res_edqy :=
-      parity_scale_codec.codec.Decode.decode __codec_input_edqy in
+      (parity_scale_codec.codec.Decode.decode
+          (Self := ink.codegen.dispatch.info.ContractCallBuilder.Type_))
+        __codec_input_edqy in
     let* α0 :=
       match __codec_res_edqy with
       | core.result.Result.Err e =>
@@ -4976,7 +5199,9 @@ Module Impl_core_cmp_PartialEq_for_erc20_erc20_Erc20Ref.
     Notation.dot := eq;
   }.
   
-  Global Instance I : core.cmp.PartialEq.Trait Self (Rhs := None) := {
+  Global Instance I
+    : core.cmp.PartialEq.Trait Self (Rhs := core.cmp.PartialEq.Default.Rhs Self)
+      := {
     core.cmp.PartialEq.eq `{H' : State.Trait} := eq;
   }.
   Global Hint Resolve I : core.
@@ -5077,7 +5302,10 @@ Module Impl_ink_storage_traits_layout_StorageLayout_for_erc20_erc20_Erc20Ref.
       `{H' : State.Trait}
       (__key : ref ink_primitives.key.Key)
       : M (H := H') ink_metadata.layout.Layout :=
-    let* α0 := ink_storage_traits.layout.StorageLayout.layout __key in
+    let* α0 :=
+      (ink_storage_traits.layout.StorageLayout.layout
+          (Self := ink.codegen.dispatch.info.ContractCallBuilder.Type_))
+        __key in
     let* α1 := ink_metadata.layout.FieldLayout::["new"] "inner" α0 in
     let* α2 := ink_metadata.layout.StructLayout::["new"] "Erc20Ref" [ α1 ] in
     Pure (ink_metadata.layout.Layout.Struct α2).
@@ -5146,7 +5374,7 @@ Module
     Context {E : Set}.
     Definition Self := core.result.Result erc20.erc20.Erc20 E.
     
-    Definition IS_RESULT := Pure true.
+    Definition IS_RESULT `{H' : State.Trait} := Pure true.
     
     Global Instance AssociatedFunction_IS_RESULT `{H' : State.Trait} :
       Notation.DoubleColon Self "IS_RESULT" := {
@@ -5263,7 +5491,9 @@ Module Impl_erc20_erc20_Erc20Ref_26.
       `{H' : State.Trait}
       (self : ref Self)
       : M (H := H') (ink_primitives.MessageResult erc20.erc20.Balance) :=
-    let* α0 := ink.codegen.trait_def.call_builder.TraitCallBuilder.call self in
+    let* α0 :=
+      (ink.codegen.trait_def.call_builder.TraitCallBuilder.call (Self := Self))
+        self in
     let* α1 := α0.["total_supply"] in
     let* α2 := α1.["try_invoke"] in
     α2.["unwrap_or_else"]
@@ -5306,7 +5536,9 @@ Module Impl_erc20_erc20_Erc20Ref_26.
       (self : ref Self)
       (owner : erc20.erc20.AccountId)
       : M (H := H') (ink_primitives.MessageResult erc20.erc20.Balance) :=
-    let* α0 := ink.codegen.trait_def.call_builder.TraitCallBuilder.call self in
+    let* α0 :=
+      (ink.codegen.trait_def.call_builder.TraitCallBuilder.call (Self := Self))
+        self in
     let* α1 := α0.["balance_of"] owner in
     let* α2 := α1.["try_invoke"] in
     α2.["unwrap_or_else"]
@@ -5350,7 +5582,9 @@ Module Impl_erc20_erc20_Erc20Ref_26.
       (owner : erc20.erc20.AccountId)
       (spender : erc20.erc20.AccountId)
       : M (H := H') (ink_primitives.MessageResult erc20.erc20.Balance) :=
-    let* α0 := ink.codegen.trait_def.call_builder.TraitCallBuilder.call self in
+    let* α0 :=
+      (ink.codegen.trait_def.call_builder.TraitCallBuilder.call (Self := Self))
+        self in
     let* α1 := α0.["allowance"] owner spender in
     let* α2 := α1.["try_invoke"] in
     α2.["unwrap_or_else"]
@@ -5395,7 +5629,9 @@ Module Impl_erc20_erc20_Erc20Ref_26.
       (value : erc20.erc20.Balance)
       : M (H := H') (ink_primitives.MessageResult (erc20.erc20.Result unit)) :=
     let* α0 :=
-      ink.codegen.trait_def.call_builder.TraitCallBuilder.call_mut self in
+      (ink.codegen.trait_def.call_builder.TraitCallBuilder.call_mut
+          (Self := Self))
+        self in
     let* α1 := α0.["transfer"] to value in
     let* α2 := α1.["try_invoke"] in
     α2.["unwrap_or_else"]
@@ -5440,7 +5676,9 @@ Module Impl_erc20_erc20_Erc20Ref_26.
       (value : erc20.erc20.Balance)
       : M (H := H') (ink_primitives.MessageResult (erc20.erc20.Result unit)) :=
     let* α0 :=
-      ink.codegen.trait_def.call_builder.TraitCallBuilder.call_mut self in
+      (ink.codegen.trait_def.call_builder.TraitCallBuilder.call_mut
+          (Self := Self))
+        self in
     let* α1 := α0.["approve"] spender value in
     let* α2 := α1.["try_invoke"] in
     α2.["unwrap_or_else"]
@@ -5488,7 +5726,9 @@ Module Impl_erc20_erc20_Erc20Ref_26.
       (value : erc20.erc20.Balance)
       : M (H := H') (ink_primitives.MessageResult (erc20.erc20.Result unit)) :=
     let* α0 :=
-      ink.codegen.trait_def.call_builder.TraitCallBuilder.call_mut self in
+      (ink.codegen.trait_def.call_builder.TraitCallBuilder.call_mut
+          (Self := Self))
+        self in
     let* α1 := α0.["transfer_from"] from to value in
     let* α2 := α1.["try_invoke"] in
     α2.["unwrap_or_else"]
@@ -5558,7 +5798,9 @@ Module Impl_ink_env_call_create_builder_FromAccountId_for_erc20_erc20_Erc20Ref.
       (account_id : erc20.erc20.AccountId)
       : M (H := H') Self :=
     let* α0 :=
-      ink_env.call.create_builder.FromAccountId.from_account_id account_id in
+      (ink_env.call.create_builder.FromAccountId.from_account_id
+          (Self := ink.codegen.dispatch.info.ContractCallBuilder.Type_))
+        account_id in
     Pure {| Self.inner := α0; |}.
   
   Global Instance AssociatedFunction_from_account_id `{H' : State.Trait} :
@@ -5585,7 +5827,9 @@ Module Impl_ink_contract_ref_ToAccountId_for_erc20_erc20_Erc20Ref.
       `{H' : State.Trait}
       (self : ref Self)
       : M (H := H') erc20.erc20.AccountId :=
-    ink.contract_ref.ToAccountId.to_account_id (addr_of self.["inner"]).
+    (ink.contract_ref.ToAccountId.to_account_id
+        (Self := ink.codegen.dispatch.info.ContractCallBuilder.Type_))
+      (addr_of self.["inner"]).
   
   Global Instance Method_to_account_id `{H' : State.Trait} :
     Notation.Dot "to_account_id" := {
@@ -5609,7 +5853,7 @@ Module Impl_core_convert_AsRef_for_erc20_erc20_Erc20Ref.
       `{H' : State.Trait}
       (self : ref Self)
       : M (H := H') (ref erc20.erc20.AccountId) :=
-    core.convert.AsRef.as_ref (addr_of self.["inner"]).
+    (core.convert.AsRef.as_ref (Self := _)) (addr_of self.["inner"]).
   
   Global Instance Method_as_ref `{H' : State.Trait} : Notation.Dot "as_ref" := {
     Notation.dot := as_ref;
@@ -5629,7 +5873,7 @@ Module Impl_core_convert_AsMut_for_erc20_erc20_Erc20Ref.
       `{H' : State.Trait}
       (self : mut_ref Self)
       : M (H := H') (mut_ref erc20.erc20.AccountId) :=
-    core.convert.AsMut.as_mut (addr_of self.["inner"]).
+    (core.convert.AsMut.as_mut (Self := _)) (addr_of self.["inner"]).
   
   Global Instance Method_as_mut `{H' : State.Trait} : Notation.Dot "as_mut" := {
     Notation.dot := as_mut;
@@ -5647,10 +5891,15 @@ Definition __ink_generate_metadata
     : M (H := H') ink_metadata.InkProject :=
   let* layout :=
     let* α0 :=
-      core.convert.From.from ink_storage_traits.storage.StorageKey.KEY in
+      (core.convert.From.from (Self := ink_metadata.layout.LayoutKey))
+        (ink_storage_traits.storage.StorageKey.KEY
+          (Self := erc20.erc20.Erc20)) in
     let* α1 :=
-      ink_storage_traits.layout.StorageLayout.layout
-        (addr_of ink_storage_traits.storage.StorageKey.KEY) in
+      (ink_storage_traits.layout.StorageLayout.layout
+          (Self := erc20.erc20.Erc20))
+        (addr_of
+          (ink_storage_traits.storage.StorageKey.KEY
+            (Self := erc20.erc20.Erc20))) in
     let* α2 := ink_metadata.layout.RootLayout::["new"] α0 α1 in
     Pure (ink_metadata.layout.Layout.Root α2) in
   let* _ :=
@@ -5679,7 +5928,11 @@ Definition __ink_generate_metadata
   let* α10 := α9.["payable"] false in
   let* α11 := α10.["default"] false in
   let* α12 :=
-    if (ink.reflect.dispatch.DispatchableConstructorInfo.IS_RESULT : bool) then
+    if
+      (ink.reflect.dispatch.DispatchableConstructorInfo.IS_RESULT
+        (Self := erc20.erc20.Erc20)
+      : bool)
+    then
       let* α0 :=
         ink_metadata.specs.TypeSpec::["with_name_str"]
           "ink_primitives::ConstructorResult" in
@@ -6139,7 +6392,9 @@ Module Impl_core_cmp_PartialEq_for_erc20_erc20_Error.
     Notation.dot := eq;
   }.
   
-  Global Instance I : core.cmp.PartialEq.Trait Self (Rhs := None) := {
+  Global Instance I
+    : core.cmp.PartialEq.Trait Self (Rhs := core.cmp.PartialEq.Default.Rhs Self)
+      := {
     core.cmp.PartialEq.eq `{H' : State.Trait} := eq;
   }.
   Global Hint Resolve I : core.
@@ -6211,7 +6466,8 @@ Module Impl_parity_scale_codec_encode_like_EncodeLike_for_erc20_erc20_Error.
   Definition Self := erc20.erc20.Error.
   
   Global Instance I
-    : parity_scale_codec.encode_like.EncodeLike.Trait Self (T := None)
+    : parity_scale_codec.encode_like.EncodeLike.Trait Self
+        (T := parity_scale_codec.encode_like.EncodeLike.Default.T Self)
       := parity_scale_codec.encode_like.EncodeLike.Build_Trait _.
   Global Hint Resolve I : core.
 End Impl_parity_scale_codec_encode_like_EncodeLike_for_erc20_erc20_Error.
@@ -6263,7 +6519,7 @@ Module Impl_parity_scale_codec_codec_Decode_for_erc20_erc20_Error.
         let* α0 :=
           (fun  =>
               let* α0 :=
-                core.convert.Into.into
+                (core.convert.Into.into (Self := _))
                   "Could not decode `Error`, variant doesn't exist" in
               Pure (core.result.Result.Err α0)) in
         Return α0 in
