coq_translation/default/examples/generics/generics_phantom_type.v
@@ -55,7 +55,10 @@ Module Impl_core_cmp_PartialEq_for_generics_phantom_type_PhantomTuple_A_B.
       Notation.dot := eq;
     }.
     
-    Global Instance I : core.cmp.PartialEq.Trait Self (Rhs := None) := {
+    Global Instance I
+      : core.cmp.PartialEq.Trait Self
+          (Rhs := core.cmp.PartialEq.Default.Rhs Self)
+        := {
       core.cmp.PartialEq.eq `{H' : State.Trait} := eq;
     }.
   End Impl_core_cmp_PartialEq_for_generics_phantom_type_PhantomTuple_A_B.
@@ -122,7 +125,10 @@ Module Impl_core_cmp_PartialEq_for_generics_phantom_type_PhantomStruct_A_B.
       Notation.dot := eq;
     }.
     
-    Global Instance I : core.cmp.PartialEq.Trait Self (Rhs := None) := {
+    Global Instance I
+      : core.cmp.PartialEq.Trait Self
+          (Rhs := core.cmp.PartialEq.Default.Rhs Self)
+        := {
       core.cmp.PartialEq.eq `{H' : State.Trait} := eq;
     }.
   End Impl_core_cmp_PartialEq_for_generics_phantom_type_PhantomStruct_A_B.
