coq_translation/default/examples/traits/derive.v
@@ -37,7 +37,9 @@ Module Impl_core_cmp_PartialEq_for_derive_Centimeters.
     Notation.dot := eq;
   }.
   
-  Global Instance I : core.cmp.PartialEq.Trait Self (Rhs := None) := {
+  Global Instance I
+    : core.cmp.PartialEq.Trait Self (Rhs := core.cmp.PartialEq.Default.Rhs Self)
+      := {
     core.cmp.PartialEq.eq `{H' : State.Trait} := eq;
   }.
   Global Hint Resolve I : core.
@@ -58,7 +60,10 @@ Module Impl_core_cmp_PartialOrd_for_derive_Centimeters.
     Notation.dot := partial_cmp;
   }.
   
-  Global Instance I : core.cmp.PartialOrd.Trait Self (Rhs := None) := {
+  Global Instance I
+    : core.cmp.PartialOrd.Trait Self
+        (Rhs := core.cmp.PartialOrd.Default.Rhs Self)
+      := {
     core.cmp.PartialOrd.partial_cmp `{H' : State.Trait} := partial_cmp;
   }.
   Global Hint Resolve I : core.
